theories/heap_lang/lib/spin_lock.v
@@ -60,7 +60,7 @@ Section proof.
     {{{ is_lock γ lk R }}} try_acquire lk
     {{{ b, RET #b; if b is true then locked γ ∗ R else True }}}.
   Proof.
-    iIntros (Φ) "#Hl HΦ". iDestruct "Hl" as (l) "[% #?]"; subst.
+    iIntros (Φ) "#Hl HΦ". iDestruct "Hl" as (l ->) "#Hinv".
     wp_rec. iInv N as ([]) "[Hl HR]" "Hclose".
     - wp_cas_fail. iMod ("Hclose" with "[Hl]"); first (iNext; iExists true; eauto).
       iModIntro. iApply ("HΦ" $! false). done.
@@ -82,7 +82,7 @@ Section proof.
     {{{ is_lock γ lk R ∗ locked γ ∗ R }}} release lk {{{ RET #(); True }}}.
   Proof.
     iIntros (Φ) "(Hlock & Hlocked & HR) HΦ".
-    iDestruct "Hlock" as (l) "[% #?]"; subst.
+    iDestruct "Hlock" as (l ->) "#Hinv".
     rewrite /release /=. wp_let. iInv N as (b) "[Hl _]" "Hclose".
     wp_store. iApply "HΦ". iApply "Hclose". iNext. iExists false. by iFrame.
   Qed.
