theories/program_logic/ownp.v
@@ -89,7 +89,7 @@ Section lifting.
       iMod "H" as (σ1) "[Hred _]"; iDestruct "Hred" as %Hred%reducible_not_val.
       move: Hred; by rewrite to_of_val.
     - iApply wp_lift_step; [done|]; iIntros (σ1) "Hσ".
-      iMod "H" as (σ1') "(% & >Hσf & H)". rewrite /ownP.
+      iMod "H" as (σ1' ?) "[>Hσf H]". rewrite /ownP.
       iDestruct (own_valid_2 with "Hσ Hσf")
         as %[->%Excl_included%leibniz_equiv _]%auth_valid_discrete_2.
       iModIntro; iSplit; [done|]; iNext; iIntros (e2 σ2 efs Hstep).
@@ -169,7 +169,7 @@ Section ectx_lifting.
     ⊢ WP e1 @ E {{ Φ }}.
   Proof.
     iIntros "H". iApply (ownP_lift_step E); try done.
-    iMod "H" as (σ1) "(%&Hσ1&Hwp)". iModIntro. iExists σ1.
+    iMod "H" as (σ1 ?) "[Hσ1 Hwp]". iModIntro. iExists σ1.
     iSplit; first by eauto. iFrame. iNext. iIntros (e2 σ2 efs) "% ?".
     iApply ("Hwp" with "[]"); eauto.
   Qed.
